Manual/BasicTypes.lean
@@ -131,7 +131,7 @@ tag := "char-runtime"
 %%%
 
 
-In monomorphic contexts, characters are represented as 32-bit immediate values. In other words, a field of a constructor or structure of type `Char` does not require indirection to access. In polymorphic contexts, characters are boxed.
+In monomorphic contexts, characters are represented as 32-bit immediate values. In other words, a field of a constructor or structure of type {lean}`Char` does not require indirection to access. In polymorphic contexts, characters are boxed.
 
 
 ## API Reference
