Manual/Language/RecursiveDefs.lean
@@ -1,0 +1,111 @@
+/-
+Copyright (c) 2024 Lean FRO LLC. All rights reserved.
+Released under Apache 2.0 license as described in the file LICENSE.
+Author: David Thrane Christiansen
+-/
+
+import VersoManual
+
+import Manual.Meta
+
+import Manual.Language.RecursiveDefs.Structural
+
+open Verso.Genre Manual
+open Lean.Elab.Tactic.GuardMsgs.WhitespaceMode
+
+set_option maxRecDepth 1500
+
+#doc (Manual) "Recursive Definitions" =>
+%%%
+tag := "recursive-definitions"
+%%%
+
+Allowing arbitrary recursive function definitions would make Lean's logic inconsistent.
+General recursion makes it possible to write circular proofs: "{tech}[proposition] $P$ is true because proposition $P$ is true".
+Outside of proofs, an infinite loop could be assigned the type {name}`Empty`, which can be used with {keywordOf Lean.Parser.Term.nomatch}`nomatch` or {name Empty.rec}`Empty.rec` to prove any theorem.
+
+Banning recursive function definitions outright would render Lean far less useful: {tech}[inductive types] are key to defining both predicates and data, and they have a recursive structure.
+Furthermore, most useful recursive functions do not threaten soundness, and infinite loops usually indicate mistakes in definitions rather than intentional behavior.
+Instead of banning recursive functions, Lean requires that each recursive function is defined safely.
+While elaborating recursive definitions, the Lean elaborator also produces a justification that the function being defined is safe.{margin}[The section on {ref "elaboration-results"}[the elaborator's output] in the overview of elaboration contextualizes the elaboration of recursive definitions in the overall context of the elaborator.]
+
+There are four main kinds of recursive functions that can be defined:
+
+: Structurally recursive functions
+
+  Structurally recursive functions take an argument such that the function makes recursive calls only on strict sub-components of said argument.{margin}[Strictly speaking, arguments whose types are {tech}[indexed families] are grouped together with their indices, with the whole collection considered as a unit.]
+  The elaborator translates the recursion into uses of the argument's {tech}[recursor].
+  Because every type-correct use of a recursor is guaranteed to avoid infinite regress, this translation is evidence that the function terminates.
+  Applications of functions defined via recursors are definitionally equal to the result of the recursion, and are typically relatively efficient inside the kernel.
+
+: Recursion over well-founded relations
+
+  Many functions are also difficult to convert to structural recursion; for instance, a function may terminate because the difference between an array index and the size of the array decreases as the index increases, but {name}`Nat.rec` isn't applicable because the index that increases is the function's argument.
+  Here, there is a {tech}[measure] of termination that decreases at each recursive call, but the measure is not itself an argument to the function.
+  In these cases, {tech}[well-founded recursion] can be used to define the function.
+  Well-founded recursion is a technique for systematically transforming recursive functions with a decreasing measure into recursive functions over proofs that every sequence of reductions to the measure eventually terminates at a minimum.
+  Applications of functions defined via well-founded recursion are not necessarily definitionally equal to their return values, but this equality can be proved as a proposition.
+  Even when definitional equalities exist, these functions are frequently slow to compute with because they require reducing proof terms that are often very large.
+
+: Partial functions with nonempty ranges
+
+  For many applications, it's not important to reason about the implementation of certain functions.
+  A recursive function might be used only as part of the implementation of proof automation steps, or it might be an ordinary program that will never be formally proved correct.
+  In these cases, the Lean kernel does not need either definitional or propositional equalities to hold for the definition; it suffices that soundness is maintained.
+  Functions marked {keywordOf Lean.Parser.Command.declaration}`partial` are treated as opaque constants by the kernel and are neither unfolded nor reduced.
+  All that is required for soundness is that their return type is inhabited.
+  Partial functions may still be used in compiled code as usual, and they may appear in propositions and proofs; their equational theory in Lean's logic is simply very weak.
+
+: Unsafe recursive definitions
+
+  Unsafe definitions have none of the restrictions of partial definitions.
+  They may freely make use of general recursion, and they may use features of Lean that break assumptions about its equational theory, such as primitives for casting ({name}`unsafeCast`), checking pointer equality ({name}`ptrAddrUnsafe`), and observing {tech}[reference counts] ({name}`isExclusiveUnsafe`).
+  However, any declaration that refers to an unsafe definition must itself be marked {keywordOf Lean.Parser.Command.declaration}`unsafe`, making it clear when logical soundness is not guaranteed.
+  Unsafe operations can be used to replace the implementations of other functions with more efficient variants in compiled code, while the kernel still uses the original definition.
+  The replaced function may be opaque, which results in the function name having a trivial equational theory in the logic, or it may be an ordinary function, in which case the function is used in the logic.
+  Use this feature with care: logical soundness is not at risk, but the behavior of programs written in Lean may diverge from their verified logical models if the unsafe implementation is incorrect.
+
+
+As described in the {ref "elaboration-results"}[overview of the elaborator's output], elaboration of recursive functions proceeds in two phases:
+ 1. The definition is elaborated as if Lean's core type theory had recursive definitions.
+    Aside from using recursion, this provisional definition is fully elaborated.
+    The compiler generates code from these provisional definitions.
+
+ 2. A termination analysis attempts to use the four techniques to justify the function to Lean's kernel.
+    If the definition is marked {keywordOf Lean.Parser.Command.declaration}`unsafe` or {keywordOf Lean.Parser.Command.declaration}`partial`, then that technique is used.
+    If an explicit {keywordOf Lean.Parser.Command.declaration}`termination_by` clause is present, then the indicated technique is the only one attempted.
+    If there is no such clause, then the elaborator performs a search, testing each parameter to the function as a candidate for structural recursion, and attempting to find a measure with a well-founded relation that decreases at each recursive call.
+
+This section describes the four techniques in detail.
+
+{include 0 Manual.Language.RecursiveDefs.Structural}
+
+# Well-Founded Recursion
+%%%
+tag := "well-founded-recursion"
+%%%
+
+::: planned 57
+This section will describe the translation of {deftech}[well-founded recursion].
+:::
+
+# Controlling Reduction
+
+:::planned 58
+This section will describe {deftech}_reducibility_: {deftech}[reducible], {deftech}[semi-reducible], and {deftech}[irreducible] definitions.
+:::
+
+# Partial and Unsafe Recursive Definitions
+%%%
+tag := "partial-unsafe"
+%%%
+
+:::planned 59
+This section will describe `partial` and `unsafe` definitions:
+
+
+ * Interaction with the kernel and elaborator
+ * What guarantees are there, and what aren't there?
+ * How to bridge from unsafe to safe code?
+
+:::
