Manual/Language/RecursiveDefs/Structural/CourseOfValuesExample.lean
@@ -1,0 +1,169 @@
+/-
+Copyright (c) 2024 Lean FRO LLC. All rights reserved.
+Released under Apache 2.0 license as described in the file LICENSE.
+Author: David Thrane Christiansen
+-/
+
+import VersoManual
+
+import Manual.Meta
+
+
+open Verso.Genre Manual
+open Lean.Elab.Tactic.GuardMsgs.WhitespaceMode
+
+#doc (Manual) "Recursion Example (for inclusion elsewhere)" =>
+
+
+:::example "Course-of-Values Tables"
+This definition is equivalent to {name}`List.below`:
+```lean
+def List.below' {α : Type u} {motive : List α → Sort u} : List α → Sort (max 1 u)
+  | [] => PUnit
+  | _ :: xs => motive xs ×' xs.below' (motive := motive)
+```
+
+```lean (show := false)
+theorem List.below_eq_below' : @List.below = @List.below' := by
+  funext α motive xs
+  induction xs <;> simp [List.below, below']
+  congr
+```
+
+In other words, for a given {tech}[motive], {lean}`List.below'` is a type that contains a realization of the motive for all suffixes of the list.
+
+More recursive arguments require further nested iterations of the product type.
+For instance, binary trees have two recursive occurrences.
+```lean
+inductive Tree (α : Type u) : Type u where
+  | leaf
+  | branch (left : Tree α) (val : α) (right : Tree α)
+```
+
+It's corresponding course-of-values table contains the realizations of the motive for all subtrees:
+```lean
+def Tree.below' {α : Type u} {motive : Tree α → Sort u} : Tree α → Sort (max 1 u)
+  | .leaf => PUnit
+  | .branch left _val right =>
+    motive left ×' motive right ×'
+    left.below' (motive := motive) ×'
+    right.below' (motive := motive)
+```
+
+```lean (show := false)
+theorem Tree.below_eq_below' : @Tree.below = @Tree.below' := by
+  funext α motive t
+  induction t <;> simp [Tree.below, below']
+  congr
+```
+
+For both lists and trees, the `brecOn` operator expects just a single case, rather than one per constructor.
+This case accepts a list or tree along with a table of results for all smaller values; from this, it should satisfy the motive for the provided value.
+Dependent case analysis of the provided value automatically refines the type of the memo table, providing everything needed.
+
+The following definitions are equivalent to {name}`List.brecOn` and {name}`Tree.brecOn`, respectively.
+The primitive recursive helpers {name}`List.brecOnTable`  and {name}`Tree.brecOnTable` compute the course-of-values tables along with the final results, and the actual definitions of the `brecOn` operators simply project out the result.
+```lean
+def List.brecOnTable {α : Type u}
+    {motive : List α → Sort u}
+    (xs : List α)
+    (step :
+      (ys : List α) →
+      ys.below' (motive := motive) →
+      motive ys) :
+    motive xs ×' xs.below' (motive := motive) :=
+  match xs with
+  | [] => ⟨step [] PUnit.unit, PUnit.unit⟩
+  | x :: xs =>
+    let res := xs.brecOnTable (motive := motive) step
+    let val := step (x :: xs) res
+    ⟨val, res⟩
+```
+
+```lean
+def Tree.brecOnTable {α : Type u}
+    {motive : Tree α → Sort u}
+    (t : Tree α)
+    (step :
+      (ys : Tree α) →
+      ys.below' (motive := motive) →
+      motive ys) :
+    motive t ×' t.below' (motive := motive) :=
+  match t with
+  | .leaf => ⟨step .leaf PUnit.unit, PUnit.unit⟩
+  | .branch left val right =>
+    let resLeft := left.brecOnTable (motive := motive) step
+    let resRight := right.brecOnTable (motive := motive) step
+    let branchRes := ⟨resLeft.1, resRight.1, resLeft.2, resRight.2⟩
+    let val := step (.branch left val right) branchRes
+    ⟨val, branchRes⟩
+```
+
+```lean
+def List.brecOn' {α : Type u}
+    {motive : List α → Sort u}
+    (xs : List α)
+    (step :
+      (ys : List α) →
+      ys.below' (motive := motive) →
+      motive ys) :
+    motive xs :=
+  (xs.brecOnTable (motive := motive) step).1
+```
+
+```lean
+def Tree.brecOn' {α : Type u}
+    {motive : Tree α → Sort u}
+    (t : Tree α)
+    (step :
+      (ys : Tree α) →
+      ys.below' (motive := motive) →
+      motive ys) :
+    motive t :=
+  (t.brecOnTable (motive := motive) step).1
+```
+
+```lean (show := false)
+-- Proving the above-claimed equivalence is too time consuming, but evaluating a few examples will at least catch silly mistakes!
+
+/--
+info: fun motive x y z step =>
+  step [x, y, z]
+    ⟨step [y, z] ⟨step [z] ⟨step [] PUnit.unit, PUnit.unit⟩, step [] PUnit.unit, PUnit.unit⟩,
+      step [z] ⟨step [] PUnit.unit, PUnit.unit⟩, step [] PUnit.unit, PUnit.unit⟩
+-/
+#guard_msgs in
+#reduce fun motive x y z step => List.brecOn' (motive := motive) [x, y, z] step
+
+/--
+info: fun motive x y z step =>
+  step [x, y, z]
+    ⟨step [y, z] ⟨step [z] ⟨step [] PUnit.unit, PUnit.unit⟩, step [] PUnit.unit, PUnit.unit⟩,
+      step [z] ⟨step [] PUnit.unit, PUnit.unit⟩, step [] PUnit.unit, PUnit.unit⟩
+-/
+#guard_msgs in
+#reduce fun motive x y z step => List.brecOn (motive := motive) [x, y, z] step
+
+/--
+info: fun motive x z step =>
+  step ((Tree.leaf.branch x Tree.leaf).branch z Tree.leaf)
+    ⟨step (Tree.leaf.branch x Tree.leaf) ⟨step Tree.leaf PUnit.unit, step Tree.leaf PUnit.unit, PUnit.unit, PUnit.unit⟩,
+      step Tree.leaf PUnit.unit, ⟨step Tree.leaf PUnit.unit, step Tree.leaf PUnit.unit, PUnit.unit, PUnit.unit⟩,
+      PUnit.unit⟩
+-/
+#guard_msgs in
+#reduce fun motive x z step => Tree.brecOn' (motive := motive) (.branch (.branch .leaf x .leaf) z .leaf) step
+
+/--
+info: fun motive x z step =>
+  step ((Tree.leaf.branch x Tree.leaf).branch z Tree.leaf)
+    ⟨⟨step (Tree.leaf.branch x Tree.leaf)
+          ⟨⟨step Tree.leaf PUnit.unit, PUnit.unit⟩, step Tree.leaf PUnit.unit, PUnit.unit⟩,
+        ⟨step Tree.leaf PUnit.unit, PUnit.unit⟩, step Tree.leaf PUnit.unit, PUnit.unit⟩,
+      step Tree.leaf PUnit.unit, PUnit.unit⟩
+-/
+#guard_msgs in
+#reduce fun motive x z step => Tree.brecOn (motive := motive) (.branch (.branch .leaf x .leaf) z .leaf) step
+```
+
+:::
