Manual/Language/RecursiveDefs/Structural/RecursorExample.lean
@@ -1,0 +1,120 @@
+/-
+Copyright (c) 2024 Lean FRO LLC. All rights reserved.
+Released under Apache 2.0 license as described in the file LICENSE.
+Author: David Thrane Christiansen
+-/
+
+import VersoManual
+
+import Manual.Meta
+
+
+open Verso.Genre Manual
+open Lean.Elab.Tactic.GuardMsgs.WhitespaceMode
+
+
+#doc (Manual) "Recursion Example (for inclusion elsewhere)" =>
+
+
+```lean (show := false)
+section
+variable (n k : Nat) (mot : Nat → Sort u)
+```
+:::example "Recursion vs Recursors"
+Addition of natural numbers can be defined via recursion on the second argument.
+This function is straightforwardly structurally recursive.
+```lean
+def add (n : Nat) : Nat → Nat
+  | .zero => n
+  | .succ k => .succ (add n k)
+```
+
+Defined using {name}`Nat.rec`, it is much further from the notations that most people are used to.
+```lean
+def add' (n : Nat) :=
+  Nat.rec (motive := fun _ => Nat)
+    n
+    (fun k soFar => .succ soFar)
+```
+
+Structural recursive calls made on data that isn't the immediate child of the function parameter requires either creativity or a complex yet systematic encoding.
+```lean
+def half : Nat → Nat
+  | 0 | 1 => 0
+  | n + 2 => half n + 1
+```
+One way to think about this function is as a structural recursion that flips a bit at each call, only incrementing the result when the bit is set.
+```lean
+def helper : Nat → Bool → Nat :=
+  Nat.rec (motive := fun _ => Bool → Nat)
+    (fun _ => 0)
+    (fun _ soFar =>
+      fun b =>
+        (if b then Nat.succ else id) (soFar !b))
+
+def half' (n : Nat) : Nat := helper n false
+```
+```lean (name := halfTest)
+#eval [0, 1, 2, 3, 4, 5, 6, 7, 8].map half'
+```
+```leanOutput halfTest
+[0, 0, 1, 1, 2, 2, 3, 3, 4]
+```
+
+Instead of creativity, a general technique called {deftech}[course-of-values recursion] can be used.
+Course-of-values recursion uses helpers that can be systematically derived for every inductive type, defined in terms of the recursor; Lean derives them automatically.
+For every {lean}`Nat` {lean}`n`, the type {lean}`n.below (motive := mot)` provides a value of type {lean}`mot k` for all {lean}`k < n`, represented as an iterated {TODO}[xref sigma] dependent pair type.
+The course-of-values recursor {name}`Nat.brecOn` allows a function to use the result for any smaller {lean}`Nat`.
+Using it to define the function is inconvenient:
+```lean
+noncomputable def half'' (n : Nat) : Nat :=
+  Nat.brecOn n (motive := fun _ => Nat)
+    fun k soFar =>
+      match k, soFar with
+      | 0, _ | 1, _ => 0
+      | _ + 2, ⟨_, ⟨h, _⟩⟩ => h + 1
+```
+The function is marked {keywordOf Lean.Parser.Command.declaration}`noncomputable` because the compiler doesn't support generating code for course-of-values recursion, which is intended for reasoning rather that efficient code.
+The kernel can still be used to test the function, however:
+```lean (name := halfTest2)
+#reduce [0,1,2,3,4,5,6,7,8].map half''
+```
+```leanOutput halfTest2
+[0, 0, 1, 1, 2, 2, 3, 3, 4]
+```
+
+The dependent pattern matching in the body of {lean}`half''` can also be encoded using recursors (specifically, {name}`Nat.casesOn`), if necessary:
+```lean
+noncomputable def half''' (n : Nat) : Nat :=
+  n.brecOn (motive := fun _ => Nat)
+    fun k =>
+      k.casesOn
+        (motive :=
+          fun k' =>
+            (k'.below (motive := fun _ => Nat)) →
+            Nat)
+        (fun _ => 0)
+        (fun k' =>
+          k'.casesOn
+            (motive :=
+              fun k'' =>
+                (k''.succ.below (motive := fun _ => Nat)) →
+                Nat)
+            (fun _ => 0)
+            (fun _ soFar => soFar.2.1.succ))
+```
+
+This definition still works.
+```lean (name := halfTest3)
+#reduce [0,1,2,3,4,5,6,7,8].map half''
+```
+```leanOutput halfTest3
+[0, 0, 1, 1, 2, 2, 3, 3, 4]
+```
+
+However, it is now far from the original definition and it has become difficult for most people to understand.
+Recursors are an excellent logical foundation, but not an easy way to write programs or proofs.
+:::
+```lean (show := false)
+end
+```
