Manual/Meta/SpliceContents.lean
@@ -1,0 +1,36 @@
+/-
+Copyright (c) 2024 Lean FRO LLC. All rights reserved.
+Released under Apache 2.0 license as described in the file LICENSE.
+Author: David Thrane Christiansen
+-/
+
+import Verso
+import Verso.Doc.ArgParse
+import Verso.Doc.Elab.Monad
+import VersoManual
+import Verso.Code
+
+namespace Manual
+
+open Lean Elab
+open Verso ArgParse Doc Elab Genre.Manual Html Code Highlighted.WebAssets Syntax
+
+
+structure SpliceContentsConfig where
+  moduleName : Ident
+
+def SpliceContentsConfig.parse [Monad m] [MonadInfoTree m] [MonadLiftT CoreM m] [MonadEnv m] [MonadError m] : ArgParse m SpliceContentsConfig :=
+  SpliceContentsConfig.mk <$> .positional `moduleName .ident
+
+@[part_command Verso.Syntax.block_role]
+def spliceContents : PartCommand
+  | `(block|block_role{spliceContents $_args* }[ $content ]) => throwErrorAt content "Unexpected block argument"
+  | `(block|block_role{spliceContents $args*}) => do
+    let {moduleName} ← SpliceContentsConfig.parse.run (← parseArgs args)
+    let moduleIdent ←
+      mkIdentFrom moduleName <$>
+      realizeGlobalConstNoOverloadWithInfo (mkIdentFrom moduleName (docName moduleName.getId))
+    let contentsAsBlock ← ``(Block.concat (Part.content $moduleIdent))
+    PartElabM.addBlock contentsAsBlock
+  | _ =>
+    throwUnsupportedSyntax
